examples/crypto/encrypt3.fst
@@ -1,8 +1,29 @@
+(*
+   Copyright 2008-2014 Cedric Fournet, Nikhil Swamy and Microsoft Research
 
+   Licensed under the Apache License, Version 2.0 (the "License");
+   you may not use this file except in compliance with the License.
+   You may obtain a copy of the License at
+
+       http://www.apache.org/licenses/LICENSE-2.0
+
+   Unless required by applicable law or agreed to in writing, software
+   distributed under the License is distributed on an "AS IS" BASIS,
+   WITHOUT WARRANTIES OR CONDITIONS OF ANY KIND, either express or implied.
+   See the License for the specific language governing permissions and
+   limitations under the License.
+*)
+
+(* 
+   Exercising:
+    -- indexed types
+    -- existential types
+    -- and refinements, of course
+*)
 module AES (* concrete implementation of a one-block symmetric cipher *)
 open Array
 
-type bytes = MAC.bytes // TODO unclear why we need this instead of seq byte
+type bytes = seq byte // TODO unclear why we need this instead of seq byte
 type nbytes (n:nat) = b:bytes{length b == n}
 
 let blocksize = 32 (* 256 bits *)
@@ -30,30 +51,31 @@ module SymEnc (* a multi-key symmetric variant; for simplicity: (1) only using A
 type r = AES.plain
 
 (* CPA variant: *) 
-opaque type Encrypted: #p: Type -> #k: Type -> k -> MAC.bytes -> Type    (* an opaque predicate, keeping track of honest encryptions *)
-
-type cipher (p:Type) (k:Type) (key:k) = c:AES.cipher { Encrypted key c }    (* TODO why do I need explicit implicits?; NS: you don't seem to need it *)
+opaque type Encrypted: #k: Type -> p:Type -> k -> AES.bytes -> Type         (* an opaque predicate, keeping track of honest encryptions *)
+type cipher (p:Type) (k:Type) (key:k) = c:AES.cipher { Encrypted p key c }  
 
 type keyT: Type -> Type = 
   | Ideal    : p:Type -> AES.key -> i:int -> keyT p (* maybe no need to keep plain/repr around *)
   | Concrete : p:Type -> AES.key -> i:int -> keyT p  
 
 type scheme: Type -> Type =
-  | Scheme: p: Type -> k:Type -> 
+  | Scheme:  p:Type -> k:Type -> 
              keyrepr: (k -> AES.key) -> 
              keygen:  (bool -> k) ->   
              encrypt: (key:k -> p -> cipher p k key) ->
-             decrypt: (key:k -> cipher p k key -> p) -> scheme p 
+             decrypt: (key:k -> cipher p k key -> p) -> 
+             scheme p 
 
-val create: p: Type -> plain: (r -> p) -> repr: (p -> r) -> scheme p 
+
 
 type entry (p:Type) (k:Type) = 
   | Entry : key:k -> c:cipher p k key -> plain:p -> entry p k
 
-(*
+val create: p: Type -> plain: (r -> p) -> repr: (p -> r) -> scheme p 
 let create (p:Type) plain repr = 
   let c = ST.alloc 0 in
   let log : ref (list (entry p (keyT p))) = ST.alloc [] in
+
   let keygen : bool -> keyT p = fun safe ->
     let i = !c in
     c := !c + 1;
@@ -67,76 +89,77 @@ let create (p:Type) plain repr =
     | Ideal kv _ -> failwith "no way!"
     | Concrete kv _ -> kv in
 
-  let encrypt: (key:keyT p -> p -> cipher p (keyT p) key) = fun k text ->
-    let c = 
-      match k with
-      | Ideal kv _ -> let c = AES.enc kv AES.dummy in
-                        log := Entry k c text :: !log; 
-                        c
-      | Concrete kv _ -> AES.enc kv (repr text) in
-    assume (Encrypted k c); 
-    c
-   
-  in
+  let encrypt: (k:keyT p -> p -> cipher p (keyT p) k) = fun k text ->
+    match k with
+    | Ideal kv _ -> 
+       let c = AES.enc kv AES.dummy in
+       assume (Encrypted p k c); 
+       log := Entry k c text :: !log; 
+       c
+
+    | Concrete kv _ -> 
+       let rep = repr text in    (* NS: need the let-binding because repr is impure and we can't substitute it in the type of 'enc' *) 
+       let c = AES.enc kv rep in
+       assume (Encrypted p k c); 
+       c in
+    
 
   let decrypt: key:keyT p -> cipher p (keyT p) key -> p = fun k c ->
     match k with 
     | Ideal kv _ -> (match List.find (fun (Entry k' c' _) -> k=k' && c= c') !log with 
-                      | Some e -> Entry.plain e
-                      | _ -> failwith "never")
-    | Concrete kv _ -> plain (AES.dec kv c)  
-  in
+                     | Some e -> Entry.plain e
+                     | _ -> failwith "never")
+    | Concrete kv _ -> plain (AES.dec kv c)  in
 
   Scheme p (keyT p) keyrepr keygen encrypt decrypt
- *)
    
 module SampleEncrypt
 open SymEnc
-let plain (x:AES.plain) = x 
-let repr (x:AES.plain) = x 
+let plain (x:AES.plain) = x
+let repr (x:AES.plain) = x
 
 let test() =
   let p = failwith "nice bytes" in
-  let Scheme keyrepr keygen encrypt decrypt = SymEnc.create (AES.plain) plain repr in 
+  let Scheme keyrepr keygen encrypt decrypt = SymEnc.create (AES.plain) plain repr in
   let k0 = keygen true in
   let k1 = keygen true in
   let c = encrypt k0 p in
   let p' = decrypt k0 c in
-//assert( p == p');                   // this succeeds, by functional correctness
-  (* let p'' = SymEnc.decrypt k1 c in  // this rightfully triggers an error *)
+  //assert( p == p');           // this should eventually succeed, once we prove functional correctness
+  (* let p'' = decrypt k1 c in     // this rightfully triggers an error *)
   ()
 
 
-module EncryptThenMAC 
+module EncryptThenMAC
 open SymEnc
 
 type p = AES.plain
 
-let plain (x:AES.plain) = x 
-let repr (x:AES.plain) = x 
+let plain (x:AES.plain) = x
+let repr (x:AES.plain) = x
  
 let s = SymEnc.create p plain repr
-type k = Scheme.k s 
+type k = Scheme.k s
 
-type k2 = 
-  | Key:  ke:k -> MAC.pkey (SymEnc.Encrypted #p #k ke) -> k2
+type k2 =
+  | Key:  ke:k -> MAC3.pkey (SymEnc.Encrypted (Scheme.p s) ke) -> k2
 
-type cipher = (AES.cipher * MAC.tag)
+type cipher = (AES.cipher * MAC3.tag)
 
-val decrypt: key:k2 -> cipher -> option p
+val decrypt: key:k2 -> cipher -> option (Scheme.p s)
 let decrypt (Key ke ka) (c,tag) =
-  if MAC.verify ka c tag
+  if MAC3.verify ka c tag
   then Some(Scheme.decrypt s ke c)
   else None
 
 val keygen: unit -> k2
 let keygen() =
   let ke = Scheme.keygen s true in
-  let ka = MAC.keygen (SymEnc.Encrypted #p #k ke) in
+  let ka = MAC3.keygen (SymEnc.Encrypted (Scheme.p s) ke) in
   Key ke ka
 
-val encrypt: key:k2 -> plain:p -> cipher
+val encrypt: key:k2 -> plain:Scheme.p s -> cipher
 let encrypt (Key ke ka) plain =
   let c = Scheme.encrypt s ke plain in
-  (c, MAC.mac ka c)
+  (c, MAC3.mac ka c)
 
