examples/unit-tests/negative-tests.fst
@@ -155,3 +155,12 @@ let test_node_3 (l:int) (t1:tree l) (t2:tree (l + 2)) = Node (Some t1) (l + 1) (
 let bad_node_1 () = Node #0 None 1 #2 None                                              //fails: needs to be Node #1 None 1 #1 None
 let bad_node_2 (l:int) (t:tree l) = Node (Some t) l #(l + 1) None                       //fails: needs to be (l + 1) in the middle
 let bad_node_3 (l:int) (t1:tree l) (t2:tree (l + 1)) = Node (Some t1) (l + 1) (Some t2) //fails: t2 must be at least tree (l + 2)
+
+
+(* Hard to keep this one in the suite since the program fails to even --lax check *)
+(* module EscapingVariable *)
+(* assume type Good : int -> Type *)
+(* assume val enc: plain:int -> c:unit{Good plain} *)
+(* assume val repr : int -> int *)
+ 
+(* let f (text:int) = enc (repr text) //should fail; plain escapes *)
